test/Tune_Klas_SPMM.cu
@@ -48,7 +48,7 @@ int main(int argc, char **argv)
     /* Generate sparse A and dense B on host */
     float *AD = mk_dense_matrix_f32(rows, shared, density_pct);
     smatrix_f32_t A = sparsify_f32(AD, rows, shared);
-    uint32_t *row_indices = mk_row_indices(rows, A);
+    spmm_idx_t *row_indices = mk_row_indices(rows, A);
     float *B = mk_dense_matrix_f32(shared, cols, 50);
 
     printf("+ NNZ = %u (%.1f%%)\n", A.nnz,
@@ -56,7 +56,7 @@ int main(int argc, char **argv)
 
     /* Upload to device */
     smatrix_f32_t dA;
-    uint32_t *drow_indices;
+    spmm_idx_t *drow_indices;
     float *dB, *dC;
     upload_spmm_f32(rows, shared, cols, A, row_indices, B, &dA, &drow_indices,
                     &dB, &dC);
