src/lib/kuiper/Kuiper.Kernel.Stream.fsti
@@ -3,15 +3,21 @@ module Kuiper.Kernel.Stream
 
 open Pulse
 
+[@@FStar.Attributes.custard_extern "cudaStream_t";
+   FStar.Attributes.custard_c_header "kuiper.h"]
 val stream_t: Type0
 
 val stream_live (s: stream_t) : slprop
 
+[@@FStar.Attributes.custard_extern "KPR_FRESH_STREAM";
+   FStar.Attributes.custard_c_header "kuiper.h"]
 noextract
 fn fresh_stream ()
   returns s:stream_t
   ensures stream_live s
 
+[@@FStar.Attributes.custard_extern "KPR_MUST_stream_destroy";
+   FStar.Attributes.custard_c_header "kuiper.h"]
 noextract
 fn destroy_stream
   (s: stream_t)
