src/lib/kuiper/types/Kuiper.Float16.Base.fsti
@@ -5,7 +5,10 @@ module Kuiper.Float16.Base
 open Kuiper.Floating.Base
 
 new
+[@@FStar.Attributes.custard_float 16]
 val t : Type0
+
+val of_int       : Int64.t -> t
 
 val zero : t
 val one : t
@@ -15,12 +18,12 @@ val mul : t -> t -> t
 
 val lt : t -> t -> bool
 val lte : t -> t -> bool
-val eq : t -> t -> bool
+val ieee_eq : t -> t -> bool
+unfold let eq (x y : t) : bool = ieee_eq x y
 
 val sub : t -> t -> t
 val div : t -> t -> t
 
-val of_int       : Int64.t -> t
 val of_int_zero  : squash (of_int 0L == zero)
 val of_int_one   : squash (of_int 1L == one)
 
@@ -30,7 +33,11 @@ val of_literal : string -> t
 
 val kind : t -> fkind
 
+[@@FStar.Attributes.custard_extern "HLF_MAX";
+   FStar.Attributes.custard_c_header "kuiper/math.h"]
 val largest : t
+[@@FStar.Attributes.custard_extern "HLF_INFINITY";
+   FStar.Attributes.custard_c_header "kuiper/math.h"]
 val infinity : t
 
 val kind_one      : squash (kind one == Finite)
@@ -107,6 +114,8 @@ val infinity_val_spec : (x : t) ->
           (ensures lte x infinity)
           [SMTPat (lte x infinity)]
 
+[@@FStar.Attributes.custard_extern "kpr_hfmax";
+   FStar.Attributes.custard_c_header "kuiper/math.h"]
 val fmax : t -> t -> t
 
 val fmax_spec : (x : t) -> (y : t) ->
@@ -114,30 +123,84 @@ val fmax_spec : (x : t) -> (y : t) ->
           (ensures fmax x y == (if lt x y then y else x))
           [SMTPat (fmax x y)]
 
+[@@FStar.Attributes.custard_extern "hexp";
+   FStar.Attributes.custard_c_header "kuiper/math.h"]
 val fexp : t -> t
+[@@FStar.Attributes.custard_extern "hlog";
+   FStar.Attributes.custard_c_header "kuiper/math.h"]
 val flog : t -> t
+[@@FStar.Attributes.custard_extern "kpr_hsqrt";
+   FStar.Attributes.custard_c_header "kuiper/math.h"]
 val sqrt : t -> t
+[@@FStar.Attributes.custard_extern "kpr_hrsqrt";
+   FStar.Attributes.custard_c_header "kuiper/math.h"]
 val rsqrt : t -> t
+[@@FStar.Attributes.custard_extern "kpr_hsin";
+   FStar.Attributes.custard_c_header "kuiper/math.h"]
 val sin : t -> t
+[@@FStar.Attributes.custard_extern "kpr_hcos";
+   FStar.Attributes.custard_c_header "kuiper/math.h"]
 val cos : t -> t
+[@@FStar.Attributes.custard_extern "kpr_htan";
+   FStar.Attributes.custard_c_header "kuiper/math.h"]
 val tan : t -> t
+[@@FStar.Attributes.custard_extern "kpr_hasin";
+   FStar.Attributes.custard_c_header "kuiper/math.h"]
 val asin : t -> t
+[@@FStar.Attributes.custard_extern "kpr_hacos";
+   FStar.Attributes.custard_c_header "kuiper/math.h"]
 val acos : t -> t
+[@@FStar.Attributes.custard_extern "kpr_hatan";
+   FStar.Attributes.custard_c_header "kuiper/math.h"]
 val atan : t -> t
+[@@FStar.Attributes.custard_extern "kpr_hsinh";
+   FStar.Attributes.custard_c_header "kuiper/math.h"]
 val sinh : t -> t
+[@@FStar.Attributes.custard_extern "kpr_hcosh";
+   FStar.Attributes.custard_c_header "kuiper/math.h"]
 val cosh : t -> t
+[@@FStar.Attributes.custard_extern "kpr_htanh";
+   FStar.Attributes.custard_c_header "kuiper/math.h"]
 val tanh : t -> t
+[@@FStar.Attributes.custard_extern "kpr_hceil";
+   FStar.Attributes.custard_c_header "kuiper/math.h"]
 val ceil : t -> t
+[@@FStar.Attributes.custard_extern "kpr_hfloor";
+   FStar.Attributes.custard_c_header "kuiper/math.h"]
 val floor : t -> t
+[@@FStar.Attributes.custard_extern "kpr_hround";
+   FStar.Attributes.custard_c_header "kuiper/math.h"]
 val round : t -> t
+[@@FStar.Attributes.custard_extern "kpr_hfabs";
+   FStar.Attributes.custard_c_header "kuiper/math.h"]
 val fabs : t -> t
+[@@FStar.Attributes.custard_extern "kpr_herf";
+   FStar.Attributes.custard_c_header "kuiper/math.h"]
 val erf : t -> t
+[@@FStar.Attributes.custard_extern "kpr_hlog2";
+   FStar.Attributes.custard_c_header "kuiper/math.h"]
 val log2 : t -> t
+[@@FStar.Attributes.custard_extern "kpr_hlog10";
+   FStar.Attributes.custard_c_header "kuiper/math.h"]
 val log10 : t -> t
+[@@FStar.Attributes.custard_extern "kpr_hexp2";
+   FStar.Attributes.custard_c_header "kuiper/math.h"]
 val exp2 : t -> t
+[@@FStar.Attributes.custard_extern "kpr_hpow";
+   FStar.Attributes.custard_c_header "kuiper/math.h"]
 val pow : t -> t -> t
+[@@FStar.Attributes.custard_extern "kpr_hatan2";
+   FStar.Attributes.custard_c_header "kuiper/math.h"]
 val atan2 : t -> t -> t
+[@@FStar.Attributes.custard_extern "kpr_hfmin";
+   FStar.Attributes.custard_c_header "kuiper/math.h"]
 val fmin : t -> t -> t
+[@@FStar.Attributes.custard_extern "kpr_hfmod";
+   FStar.Attributes.custard_c_header "kuiper/math.h"]
 val fmod : t -> t -> t
+[@@FStar.Attributes.custard_extern "kpr_hcopysign";
+   FStar.Attributes.custard_c_header "kuiper/math.h"]
 val copysign : t -> t -> t
+[@@FStar.Attributes.custard_extern "kpr_hfma";
+   FStar.Attributes.custard_c_header "kuiper/math.h"]
 val fma : t -> t -> t -> t
